Leanbin/Init/Meta/InteractiveBase.lean
@@ -91,8 +91,8 @@ unsafe def list_of (p : parser α) :=
   brackets "[" "]" <| sep_by (skip_info (tk ",")) p
 #align interactive.types.list_of interactive.types.list_of
 
-/- ./././Mathport/Syntax/Translate/Command.lean:694:29: warning: unsupported: precedence command -/
-/- ./././Mathport/Syntax/Translate/Command.lean:694:29: warning: unsupported: precedence command -/
+/- ././././Mathport/Syntax/Translate/Command.lean:694:29: warning: unsupported: precedence command -/
+/- ././././Mathport/Syntax/Translate/Command.lean:694:29: warning: unsupported: precedence command -/
 /-- The right-binding power 2 will terminate expressions by
     '<|>' (rbp 2), ';' (rbp 1), and ',' (rbp 0). It should be used for any (potentially)
     trailing expression parameters. -/
@@ -149,7 +149,7 @@ unsafe def only_flag : parser Bool :=
 
 end Types
 
-/- ./././Mathport/Syntax/Translate/Command.lean:694:29: warning: unsupported: precedence command -/
+/- ././././Mathport/Syntax/Translate/Command.lean:694:29: warning: unsupported: precedence command -/
 open Expr Format Tactic Types
 
 private unsafe def maybe_paren : List format → format
