lakefile.lean
@@ -1,25 +1,19 @@
 import Lake
 open Lake DSL System
 
-def tag : String := "nightly-2024-05-06-08"
+def tag : String := "nightly-2024-05-10-08"
 def releaseRepo : String := "leanprover-community/mathport"
 def oleanTarName : String := "lean3-binport.tar.gz"
 
-def download (url : String) (to : FilePath) : BuildM PUnit := Lake.proc
-{ -- We use `curl -O` to ensure we clobber any existing file.
-  cmd := "curl",
-  args := #["-L", "-O", url]
-  cwd := to }
+def untar (file : FilePath) : JobM PUnit := Lake.proc
+  { cmd := "tar",
+    args := #["-xzf", file.fileName.getD "."] -- really should throw an error if `file.fileName = none`
+    cwd := file.parent }
 
-def untar (file : FilePath) : BuildM PUnit := Lake.proc
-{ cmd := "tar",
-  args := #["-xzf", file.fileName.getD "."] -- really should throw an error if `file.fileName = none`
-  cwd := file.parent }
+def getReleaseArtifact (repo tag artifact : String) (to : FilePath) : JobM PUnit :=
+  download s!"https://github.com/{repo}/releases/download/{tag}/{artifact}" to
 
-def getReleaseArtifact (repo tag artifact : String) (to : FilePath) : BuildM PUnit :=
-download s!"https://github.com/{repo}/releases/download/{tag}/{artifact}" to
-
-def untarReleaseArtifact (repo tag artifact : String) (to : FilePath) : BuildM PUnit := do
+def untarReleaseArtifact (repo tag artifact : String) (to : FilePath) : JobM PUnit := do
   getReleaseArtifact repo tag artifact to
   untar (to / artifact)
 
@@ -27,7 +21,7 @@ package lean3port where
   extraDepTargets := #[`fetchOleans]
 
 target fetchOleans (_pkg) : Unit := do
-  let libDir : FilePath := __dir__ / "build" / "lib"
+  let libDir : FilePath := __dir__ / ".lake" / "build" / "lib"
   IO.FS.createDirAll libDir
   let oldTrace := Hash.ofString tag
   let _ ← buildFileUnlessUpToDate (libDir / oleanTarName) oldTrace do
@@ -35,7 +29,7 @@ target fetchOleans (_pkg) : Unit := do
     untarReleaseArtifact releaseRepo tag oleanTarName libDir
   return .nil
 
-require mathlib from git "https://github.com/leanprover-community/mathlib4.git"@"d9f149747c04f8bb199b594ef9b689f9bbf038dd"
+require mathlib from git "https://github.com/leanprover-community/mathlib4.git"@"b72ddd8f67eba47cffd3f3422d6c01f1e666c23f"
 
 @[default_target]
 lean_lib Leanbin where
